Dafny/examples/Challenge6/Challenge6CodeLemmasPatchSideEffect.i.dfy
@@ -6,6 +6,7 @@ include "../../Libraries/Seqs.s.dfy"
 include "../../LLVM/memory.i.dfy"
 include "Challenge6Code.s.dfy"
 include "../../LLVM/Operations/binaryOperations.i.dfy"
+include "Challenge6Common.i.dfy"
 
 module challenge6CodeLemmasPatchSideEffect{
     import opened control_flow
@@ -16,15 +17,13 @@ module challenge6CodeLemmasPatchSideEffect{
     import opened memory
     import opened challenge6Code
     import opened binary_operations_i
+    import opened challenge6common
 
-// -- hechenxi@umich : chenxi
 
 lemma unwrapPatchSideEffectBehaviors(s:state, c:codeRe) returns (preB:behavior)
         requires ValidState(s);
         requires validStartingState(s);
         requires c == challenge_prob_6_code_write_encrypted_simple_patch_side_effect();
-
-        // -- input is valid -- ie. valid 16 bit integer 
         requires validInput(s);
         
         // ensures ValidBehaviorNonTrivial(preB);
@@ -32,31 +31,7 @@ lemma unwrapPatchSideEffectBehaviors(s:state, c:codeRe) returns (preB:behavior)
         ensures |preB| == 11;
         ensures preB[0] == s;
         
-        ensures StateNext(preB[0],preB[1]);
-        ensures StateNext(preB[1],preB[2]);
-        ensures ValidState(preB[0]);
-        ensures ValidState(preB[1]);
-        ensures ValidState(preB[2]);
-        ensures preB[2] == preB[3];
-        ensures ValidState(preB[3]);
-        ensures preB[3] == preB[4];
-        ensures ValidState(preB[4]);
-        ensures ValidState(preB[5]);
-        ensures StateNext(preB[0],preB[1]);
-        ensures StateNext(preB[1],preB[2]);
-        ensures StateNext(preB[2],preB[3]);
-        ensures StateNext(preB[3],preB[4]);
-        ensures StateNext(preB[4],preB[5]);
-        ensures StateNext(preB[5],preB[6]);
-        ensures ValidState(preB[6]);
-        ensures StateNext(preB[6],preB[7]);
-        ensures ValidState(preB[7]);
-        ensures StateNext(preB[7],preB[8]);
-        ensures ValidState(preB[8]);
-        ensures StateNext(preB[8],preB[9]);
-        ensures ValidState(preB[9]);
-        // ensures preB == [s] + evalCodeRE(c,s);
-        // ensures 
+       ensures validPracticalBehavior(preB);
        ensures behaviorOutput(preB) == [Nil,
                                         Nil,
                                         Nil,
@@ -91,7 +66,6 @@ lemma unwrapPatchSideEffectBehaviors(s:state, c:codeRe) returns (preB:behavior)
         var cipherText := D(Ptr(0,0,0,1));
         var bytes_written := D(Ptr(0,0,0,1));
 
-        // var c := challenge_prob_5_code_write_encrypted_simple();
          assert |c.block| == 9;
         preB := [s] + evalCodeRE(c,s);
        
@@ -146,8 +120,6 @@ lemma unwrapPatchSideEffectBehaviors(s:state, c:codeRe) returns (preB:behavior)
         assert ValidState(preB[7]);
         
         assert cmp.LV?;
-        // var r := D(Int(0,IntType(4,false)));
-        // assert  IntFits(r.d.val,r.d.itype);
         var src2 := validZero16bitInt(preB[7]);
         assert ValidOperand(preB[7],call3);// 
         assert ValidOperand(preB[7],src2);
@@ -158,11 +130,8 @@ lemma unwrapPatchSideEffectBehaviors(s:state, c:codeRe) returns (preB:behavior)
         intsTypeMatch(OperandContents(preB[7],call3),OperandContents(preB[7],src2));
         assert typesMatch(OperandContents(preB[7],call3),OperandContents(preB[7],src2));
 
-        // assert (Int(1,IntType(4,false))) == OperandContents(preB[7],call3);
         assert ValidInstruction(preB[7],ICMP(cmp,eq,4,call3,src2));
-
         assert preB[8] == evalInsRe(ICMP(cmp,eq,4,call3,src2),preB[7]);
-        // var s' := stateUpdateVar(preB[7],cmp,evalICMP(eq,4,OperandContents(preB[7],call3),OperandContents(preB[7],src2)));
 
 
         assert NextStep(preB[7],preB[8],Step.evalInsStep(ICMP(cmp,eq,4,call3,src2)));
@@ -170,17 +139,16 @@ lemma unwrapPatchSideEffectBehaviors(s:state, c:codeRe) returns (preB:behavior)
         assert ValidState(preB[8]);
 
         assert ValidInstruction(preB[8],CALL(D(Void),stateOutputDump(KEY,INTEGRITY_SIZE)));
-        // assert c[7] == CALL(D(Void),stateOutputDump(KEY,IV_SIZE));
         assert preB[9] == evalInsRe(CALL(D(Void),stateOutputDump(KEY,INTEGRITY_SIZE)),preB[8]);
         var dump := unwrapDumpWitness(preB[8],KEY,INTEGRITY_SIZE,preB[9]);
         assert NextStep(preB[8],preB[9],Step.evalInsStep(CALL(D(Void),stateOutputDump(KEY,INTEGRITY_SIZE))));   
         assert preB[9].o == SubOut([Out((Int(16,IntType(4,false)))),Out(Int(3,IntType(1,false))),Out(Int(3,IntType(1,false)))]);
 
-assert preB[9] == preB[10];
+        assert preB[9] == preB[10];
         equalStatesAreStutter(preB[9],preB[10]);
-        // assert ValidState(preB[8]);
-        // assert NextStep(preB[7],preB[8],Step.stutterStep());
         assert StateNext(preB[9],preB[10]);
+        assert validPracticalBehavior(preB);
+
 
         assert behaviorOutput(preB) == [Nil,
                                         Nil,
@@ -213,38 +181,7 @@ assert preB[9] == preB[10];
 
     }
 
-    lemma equalStatesAreStutter(s:state,s':state)
-        requires s==s'
-        requires ValidState(s);
-        ensures ValidState(s');
-        ensures NextStep(s,s',Step.stutterStep());
-        ensures StateNext(s,s');
-    {
-         assert ValidState(s');
-         assert NextStep(s,s',Step.stutterStep());
-         assert StateNext(s,s');
-    }
-
-    lemma intsTypeMatch(x:Data,y:Data)
-        requires (isInt(x) && isInt(y))
-        requires x.itype.size == y.itype.size
-        requires x.itype.signed == y.itype.signed
-        ensures typesMatch(x,y);
-    {
-        assert typesMatch(x,y);
-    }
-
-    function validZero16bitInt(s:state) : (val:operand)
-        ensures val.D?;
-        ensures val.d.Int?;
-        ensures ValidData(s, val.d)
-        ensures !val.d.itype.signed
-        ensures val.d.itype.size == 4
-    {
-        var val := D(Int(0,IntType(4,false)));
-        assert  IntFits(val.d.val,val.d.itype);
-        val
-    }
+    
 
 lemma unwrapDigestSideEffectsWitness(s:state,dst:operand,digest:operand,INTEGRITY_SIZE:operand, mblock:operand,sNext:state) returns (b:behavior)
         requires ValidState(s)
@@ -328,15 +265,13 @@ lemma unwrapDigestSideEffectsWitness(s:state,dst:operand,digest:operand,INTEGRIT
         ensures ValidBehavior(b);
         ensures |b| == 3
         ensures ValidOperand(last(b),dst)
-        // ensures OperandContents(last(b),dst) == OperandContents(s,dst);
 
         ensures ValidOperand(last(b),INTEGRITY_SIZE) && OperandContents(last(b),INTEGRITY_SIZE).Int?
         ensures OperandContents(last(b),INTEGRITY_SIZE).val == 3;
-         ensures NextStep(s,sNext,Step.evalInsStep(CALL(dst,encrypt_side_effects(INTEGRITY_SIZE))));
+        ensures NextStep(s,sNext,Step.evalInsStep(CALL(dst,encrypt_side_effects(INTEGRITY_SIZE))));
         ensures StateNext(s,sNext);
         ensures ValidState(sNext);
         ensures ValidOperand(sNext,INTEGRITY_SIZE);
-        // ensures OperandContents(s,dst) == OperandContents(last(b),dst);
         ensures sNext == last(b).(o := Nil);
         ensures behaviorOutput(b) == [Nil,Nil,Nil]
         ensures OperandContents(sNext,INTEGRITY_SIZE) == Int(3,IntType(1,false));
@@ -349,286 +284,24 @@ lemma unwrapDigestSideEffectsWitness(s:state,dst:operand,digest:operand,INTEGRIT
         assert encrypt_side_effects(INTEGRITY_SIZE) == [Ins(SUB(INTEGRITY_SIZE,1,INTEGRITY_SIZE,D(Int(1,IntType(1,false))))),CNil];
         var step,remainder,subBehavior := unwrapBlockWitness(subB,encrypt_side_effects(INTEGRITY_SIZE),s);
         step,remainder,subBehavior := unwrapBlockWitness(subBehavior,remainder,last(step));
-        // step,remainder,subBehavior := unwrapBlockWitness(subBehavior,remainder,last(step));
-         assert subB[0] == s;
-         assert subB[1] == evalInsRe(SUB(INTEGRITY_SIZE,1,INTEGRITY_SIZE,D(Int(1,IntType(1,false)))),s);
-         assert NextStep(subB[0],subB[1],Step.evalInsStep(SUB(INTEGRITY_SIZE,1,INTEGRITY_SIZE,D(Int(1,IntType(1,false))))));
-         assert subB[1] == subB[2];
+        assert subB[0] == s;
+        assert subB[1] == evalInsRe(SUB(INTEGRITY_SIZE,1,INTEGRITY_SIZE,D(Int(1,IntType(1,false)))),s);
+        assert NextStep(subB[0],subB[1],Step.evalInsStep(SUB(INTEGRITY_SIZE,1,INTEGRITY_SIZE,D(Int(1,IntType(1,false))))));
+        assert subB[1] == subB[2];
         assert subB[2] == stateUpdateVar(s,INTEGRITY_SIZE,evalSUB(1,OperandContents(s,INTEGRITY_SIZE),(Int(1,IntType(1,false)))));
         assert dst.l in subB[1].lvs;
         assert dst.l != INTEGRITY_SIZE.l;
         assert forall lv :: (lv in s.lvs && lv != INTEGRITY_SIZE.l) ==> subB[1].lvs[lv] == s.lvs[lv];
 
         assert s.lvs[dst.l] == subB[1].lvs[dst.l];
-        //  assert OperandContents(s,dst) == OperandContents(subB[1],dst);
-         equalStatesAreStutter(subB[1],subB[2]);
-         assert StateNext(subB[1],subB[2]);
-         assert |subB| == 3;
-         assert subB[2] == last(subB);
-         assert  OperandContents(subB[2],INTEGRITY_SIZE).val == 3;
-         assert ValidBehavior(subB);
-         return subB;
-    }
-
-    lemma unwrapDumpWitness(s:state,op1:operand,op2:operand,sNext:state) returns (b:behavior)
-        requires ValidState(s)
-        requires ValidOperand(s,op1)
-        requires ValidOperand(s,op2)
-        requires sNext == evalInsRe(CALL(D(Void),stateOutputDump(op1,op2)),s)
-        requires ValidInstruction(s,CALL(D(Void),stateOutputDump(op1,op2)));
-        requires s.o == Nil
-
-        ensures |b| == 4
-        ensures ValidBehavior(b);
-        ensures ValidOperand(last(b),D(Void));
-        // ensures ValidOperand(b[1],op2);
-        ensures behaviorOutput(b) == [Nil,Out(OperandContents(s,op1)),Out(OperandContents(s,op2)),Out(OperandContents(s,op2))];
-        ensures NextStep(s,sNext,Step.evalInsStep(CALL(D(Void),stateOutputDump(op1,op2))));
-        ensures StateNext(s,sNext);
-        ensures ValidState(sNext);
-        ensures sNext.o == SubOut([Out(OperandContents(s,op1)),Out(OperandContents(s,op2)),Out(OperandContents(s,op2))]);
-
-    {
-        reveal_behaviorOutput();
-        var subB := [s] + evalCodeRE(Block(stateOutputDump(op1,op2)),s);// alBlockRE(stateOutputDump(op1,op2),s);
-        assert stateOutputDump(op1,op2) == [Ins(RET((op1))),Ins(RET((op2)))];
-
-        var step,remainder,subBehavior := unwrapBlockWitness(subB,stateOutputDump(op1,op2),s);
-        step,remainder,subBehavior := unwrapBlockWitness(subBehavior,remainder,last(step));
-        step,remainder,subBehavior := unwrapBlockWitness(subBehavior,remainder,last(step));
-        
-        assert subB[0] == s;
-        assert NextStep(subB[0],subB[1],Step.evalInsStep(RET((op1))));
-        assert ValidState(subB[1]);
-        assert subB[1].o == Out(OperandContents(s,op1));
-        assert NextStep(subB[1],subB[2],Step.evalInsStep(RET((op2))));
-        assert ValidState(subB[2]);
-        assert subB[2].o == Out(OperandContents(s,op2));
-        assert subB[2] == subB[3];
-        equalStatesAreStutter(subB[2],subB[3]);
-        assert StateNext(subB[2],subB[3]);
-        assert behaviorOutput(subB) == [Nil,Out(OperandContents(s,op1)),Out(OperandContents(s,op2)),Out(OperandContents(s,op2))];
-        assert sNext == evalInsRe(CALL(D(Void),stateOutputDump(op1,op2)),s);
-        assert sNext.ok;
-        var rest := evalBlockRE(stateOutputDump(op1,op2),s);
-        assert subB == [s] + rest;
-        assert behaviorOutput(rest) == [Out(OperandContents(s,op1)),Out(OperandContents(s,op2)),Out(OperandContents(s,op2))];
-        assert sNext.o == SubOut(behaviorOutput(rest));
+        equalStatesAreStutter(subB[1],subB[2]);
+        assert StateNext(subB[1],subB[2]);
+        assert |subB| == 3;
+        assert subB[2] == last(subB);
+        assert  OperandContents(subB[2],INTEGRITY_SIZE).val == 3;
+        assert ValidBehavior(subB);
         return subB;
     }
 
-
-
-    lemma unwrapFwriteWitness(s:state,dst:operand,ptr:operand, size:nat, cnt:nat, file:operand,sNext:state) returns (b:behavior)
-        requires ValidState(s)
-        requires ValidOperand(s,ptr)
-        requires ValidOperand(s,dst)
-        requires isInt(OperandContents(s,dst));
-        requires sNext == evalInsRe(CALL(dst,fwrite(ptr,size,cnt,file)),s)
-        requires ValidInstruction(s,CALL(dst,fwrite(ptr,size,cnt,file)));
-        // ensures 
-        ensures |b| > 0
-        ensures ValidBehavior(b);
-        ensures ValidOperand(last(b),dst);
-        ensures behaviorOutput(b) == [Out(OperandContents(s,ptr)),Out(OperandContents(s,ptr))];
-        ensures b == evalBlockRE(fwrite(ptr,size,cnt,file),s);
-        ensures NextStep(s,sNext,Step.evalInsStep(CALL(dst,fwrite(ptr,size,cnt,file))));
-        ensures StateNext(s,sNext);
-        ensures ValidState(sNext);
-        ensures isInt(OperandContents(sNext,dst));
-        ensures OperandContents(sNext,dst).itype.size == OperandContents(s,dst).itype.size;
-        ensures OperandContents(sNext,dst).itype.signed == OperandContents(s,dst).itype.signed;
-
-
-    {
-        // assert ValidInstruction(s,CALL(dst,fwrite(ptr,size,cnt,file)));
-        var subB := evalBlockRE(fwrite(ptr,size,cnt,file),s);
-        assert fwrite(ptr,size,cnt,file) == [Ins(RET(ptr)),CNil];
-        var metaB := evalCodeRE(Ins(RET(ptr)),s);
-        assert ValidInstruction(s,RET(ptr));
-        assert metaB == [evalInsRe(RET(ptr),s)];
-        var s' := s.(o := Out(OperandContents(s,ptr)));
-        assert metaB == [s'];
-        assert ValidState(s');
-        var theRest := evalBlockRE([CNil],s');
-        assert theRest == [s'];
-        assert subB == [s',s'];
-        assert NextStep(subB[0],subB[1],Step.stutterStep());
-        // assert validEvalIns(ins,s,s');
-        assert sNext.ok ==> NextStep(s,sNext,Step.evalInsStep(CALL(dst,fwrite(ptr,size,cnt,file))));
-        return subB;
-    }
-
-
+    
 }
-
-//  lemma unwrapVulnBehaviors(s:state, input:operand, c:codeRe) returns (preB:behavior)
-//         requires ValidState(s);
-//         requires validStartingState(s);
-//         requires c == challenge_prob_5_code_write_encrypted_simple();
-
-//         // -- input is valid -- ie. valid 16 bit integer 
-//         requires validInput(s,input);
-        
-//         // ensures ValidBehaviorNonTrivial(preB);
-//         ensures BehaviorEvalsCode(challenge_prob_5_code_write_encrypted_simple(),preB);
-//         ensures |preB| == 9;
-//         ensures preB[0] == s;
-//                 ensures StateNext(preB[0],preB[1]);
-
-//         ensures StateNext(preB[1],preB[2]);
-//                 ensures ValidState(preB[0]);
-//         ensures ValidState(preB[1]);
-
-//         ensures ValidState(preB[2]);
-//         ensures preB[2] == preB[3];
-//         ensures ValidState(preB[3]);
-//         ensures preB[3] == preB[4];
-//         ensures ValidState(preB[4]);
-//         ensures ValidState(preB[5]);
-//         ensures StateNext(preB[0],preB[1]);
-
-//         ensures StateNext(preB[1],preB[2]);
-
-//         ensures StateNext(preB[2],preB[3]);
-
-//         ensures StateNext(preB[3],preB[4]);
-//         ensures StateNext(preB[4],preB[5]);
-
-//         ensures StateNext(preB[5],preB[6]);
-//         ensures ValidState(preB[6]);
-//         ensures StateNext(preB[6],preB[7]);
-//         ensures ValidState(preB[7]);
-//         ensures StateNext(preB[7],preB[8]);
-//         ensures ValidState(preB[8]);
-//         ensures preB == [s] + evalCodeRE(c,s);
-//         // ensures 
-//         ensures behaviorOutput(preB) == [Nil,Nil,Nil,Nil,Nil,Nil,Out(Ptr(0,0,0,1)),Nil,Nil];
-
-
-//     {
-//         reveal_BehaviorEvalsCode();
-//         // reveal_ValidBehavior();
-
-//         var call:operand := LV("call");
-//         var call1:operand := LV("call1");
-//         var mblock:operand := LV("mblock");
-//         var call2 :=LV("call2");
-//         var call3 := LV("call3");
-//                 assert OperandContents(s,call3).itype.size == 4;
-
-//         var cmp := LV("cmp");
-//         var IV_SIZE := D(Int(16,IntType(4,false)));
-//         var KEY := D(Int(16,IntType(4,false)));
-//         var cipherText := D(Ptr(0,0,0,1));
-//         var bytes_written := D(Ptr(0,0,0,1));
-
-//         // var c := challenge_prob_5_code_write_encrypted_simple();
-//         assert |c.block| == 7;
-//         preB := [s] + evalCodeRE(c,s);
-       
-//         var step,remainder,subBehavior := unwrapBlockWitness(preB,c.block,s);
-
-//             step,remainder,subBehavior := unwrapBlockWitness(subBehavior,remainder,last(step));
-//             step,remainder,subBehavior := unwrapBlockWitness(subBehavior,remainder,last(step));
-//             step,remainder,subBehavior := unwrapBlockWitness(subBehavior,remainder,last(step));
-//             step,remainder,subBehavior := unwrapBlockWitness(subBehavior,remainder,last(step));
-//             step,remainder,subBehavior := unwrapBlockWitness(subBehavior,remainder,last(step));
-//             step,remainder,subBehavior := unwrapBlockWitness(subBehavior,remainder,last(step));
-//             step,remainder,subBehavior := unwrapBlockWitness(subBehavior,remainder,last(step));
-        
-//         assert preB[0] == s;
-//         assert preB[1] == evalInsRe(CALL(call,malloc(Int(0,IntType(8,false)))),s);
-//         assert ValidOperand(preB[1],call);
-
-//         assert NextStep(preB[1],preB[2],Step.evalInsStep(LLVM_MEMCPY(call,mblock,1,false)));
-//         assert StateNext(preB[1],preB[2]);
-//         assert ValidState(preB[2]);
-//         assert preB[2] == evalInsRe(LLVM_MEMCPY(call,mblock,1,false),preB[1]);
-// // 
-//         assert preB[2] == preB[3];
-//         assert NextStep(preB[2],preB[3],Step.evalInsStep(CALL(call1,malloc(Ptr(0,0,0,1)))));
-//         assert ValidState(preB[3]);
-
-//         assert NextStep(preB[3],preB[4],Step.evalInsStep(CALL(call2,encrypt(call,4,KEY,IV_SIZE,cipherText))));
-//         assert preB[3] == preB[4];
-//         assert ValidState(preB[4]);
-        
-//         assert NextStep(preB[4],preB[5],Step.evalInsStep(STORE(call2,bytes_written)));
-//         assert ValidState(preB[5]);
-        
-
-//         assert ValidInstruction(preB[5],CALL(call3,fwrite(bytes_written,4,1,D(Ptr(0,0,0,1)))));
-//         assert preB[6] == evalInsRe(CALL(call3,fwrite(bytes_written,4,1,D(Ptr(0,0,0,1)))),preB[5]);
-//         var subB := unwrapFwriteWitness(preB[5],call3,bytes_written,4,1,D(Ptr(0,0,0,1)),preB[6]);
-
-//         assert behaviorOutput(subB) == [Out(OperandContents(preB[5],bytes_written)),Out(OperandContents(preB[5],bytes_written))];
-//         assert OperandContents(preB[5],bytes_written) == Ptr(0,0,0,1);
-//         assert ValidBehavior(subB);
-//         assert ValidOperand(last(subB),call3);
-
-//         assert NextStep(preB[5],preB[6],Step.evalInsStep(CALL(call3,fwrite(bytes_written,4,1,D(Ptr(0,0,0,1))))));
-//         // assert preB[6].ok;
-
-//         // assert preB[6].o == Out(OperandContents(preB[5],bytes_written));// == stateUpdateVar(last(subB),call3,OperandContents(last(subB),call3));
-//         assert StateNext(preB[5],preB[6]);
-//         assert ValidState(preB[6]);
-        
-//         assert cmp.LV?;
-//         // var r := D(Int(0,IntType(4,false)));
-//         // assert  IntFits(r.d.val,r.d.itype);
-//         var src2 := validZero16bitInt(preB[6]);
-//         assert ValidOperand(preB[6],call3);// 
-//         assert ValidOperand(preB[6],src2);
-//         assert && isInt(OperandContents(preB[6],call3));// 
-//         assert && isInt(OperandContents(preB[6],src2));
-//         assert OperandContents(preB[6],call3).itype.size == 4;
-//         assert !OperandContents(preB[6],call3).itype.signed;
-//         intsTypeMatch(OperandContents(preB[6],call3),OperandContents(preB[6],src2));
-//         assert typesMatch(OperandContents(preB[6],call3),OperandContents(preB[6],src2));
-
-//         // assert (Int(1,IntType(4,false))) == OperandContents(preB[6],call3);
-//         assert ValidInstruction(preB[6],ICMP(cmp,eq,4,call3,src2));
-
-//         assert preB[7] == evalInsRe(ICMP(cmp,eq,4,call3,src2),preB[6]);
-//         // var s' := stateUpdateVar(preB[6],cmp,evalICMP(eq,4,OperandContents(preB[6],call3),OperandContents(preB[6],src2)));
-
-
-//         assert NextStep(preB[6],preB[7],Step.evalInsStep(ICMP(cmp,eq,4,call3,src2)));
-//         assert StateNext(preB[6],preB[7]);
-//         assert ValidState(preB[7]);
-
-//         // // // // LAST STEP
-//         assert preB[7] == preB[8];
-//         equalStatesAreStutter(preB[7],preB[8]);
-//         // assert ValidState(preB[8]);
-//         // assert NextStep(preB[7],preB[8],Step.stutterStep());
-//         assert StateNext(preB[7],preB[8]);
-
-//         // assert ValidBehaviorNonTrivial(preB);
-//         // assert BehaviorEvalsCode(c,preB);
-//         assert |preB| == 9;
-//         assert behaviorOutput(preB) == [Nil,Nil,Nil,Nil,Nil,Nil,Out(preB[5].lvs["bytes_written"]),Nil,Nil];
-
-
-//     }
-
-    // lemma test(s:state, input:operand) returns (preB:behavior)
-    //     requires ValidState(s);
-    //     requires validStartingState(s);
-
-    //     // -- input is valid -- ie. valid 16 bit integer 
-    //     requires validInput(s,input);
-
-    // {
-    //     reveal_ValidBehavior();
-    //     reveal_BehaviorEvalsCode();
-    //     var c := challenge_prob_5_code_write_encrypted_simple();
-    //     var x := unwrapVulnBehaviors(s,input,c);
-    //     assert ValidBehaviorNonTrivial(x);
-    //     assert BehaviorEvalsCode(c,x);
-
-    //     // assert behaviorOutput(x) == [Nil,Nil,Nil,Nil,Nil,Nil,Out(x[5].lvs["bytes_written"]),Nil,Nil];
-
-    //     // assert BehaviorEvalsCode(c,preB);
-    // }
