Dafny/examples/Challenge6/Challenge6Common.i.dfy
@@ -1,0 +1,164 @@
+include "../../LLVM/llvmREFACTOR.i.dfy"
+include "../../LLVM/types.dfy"
+include "../../LLVM/control_flow.i.dfy"
+include "../../LLVM/behaviorLemmas.i.dfy"
+include "../../Libraries/Seqs.s.dfy"
+include "../../LLVM/memory.i.dfy"
+include "Challenge6Code.s.dfy"
+
+module challenge6common{
+        import opened control_flow
+        import opened LLVM_defRE
+        import opened types
+        import opened Collections__Seqs_s
+        import opened behavior_lemmas
+        import opened memory
+        import opened challenge6Code
+
+
+    lemma unwrapDumpWitness(s:state,op1:operand,op2:operand,sNext:state) returns (b:behavior)
+        requires ValidState(s)
+        requires ValidOperand(s,op1)
+        requires ValidOperand(s,op2)
+        requires sNext == evalInsRe(CALL(D(Void),stateOutputDump(op1,op2)),s)
+        requires ValidInstruction(s,CALL(D(Void),stateOutputDump(op1,op2)));
+        requires s.o == Nil
+
+        ensures |b| == 4
+        ensures ValidBehavior(b);
+        ensures ValidOperand(last(b),D(Void));
+        // ensures ValidOperand(b[1],op2);
+        ensures behaviorOutput(b) == [Nil,Out(OperandContents(s,op1)),Out(OperandContents(s,op2)),Out(OperandContents(s,op2))];
+        ensures NextStep(s,sNext,Step.evalInsStep(CALL(D(Void),stateOutputDump(op1,op2))));
+        ensures StateNext(s,sNext);
+        ensures ValidState(sNext);
+        ensures sNext.o == SubOut([Out(OperandContents(s,op1)),Out(OperandContents(s,op2)),Out(OperandContents(s,op2))]);
+
+    {
+        reveal_behaviorOutput();
+        var subB := [s] + evalCodeRE(Block(stateOutputDump(op1,op2)),s);// alBlockRE(stateOutputDump(op1,op2),s);
+        assert stateOutputDump(op1,op2) == [Ins(RET((op1))),Ins(RET((op2)))];
+
+        var step,remainder,subBehavior := unwrapBlockWitness(subB,stateOutputDump(op1,op2),s);
+        step,remainder,subBehavior := unwrapBlockWitness(subBehavior,remainder,last(step));
+        step,remainder,subBehavior := unwrapBlockWitness(subBehavior,remainder,last(step));
+        
+        assert subB[0] == s;
+        assert NextStep(subB[0],subB[1],Step.evalInsStep(RET((op1))));
+        assert ValidState(subB[1]);
+        assert subB[1].o == Out(OperandContents(s,op1));
+        assert NextStep(subB[1],subB[2],Step.evalInsStep(RET((op2))));
+        assert ValidState(subB[2]);
+        assert subB[2].o == Out(OperandContents(s,op2));
+        assert subB[2] == subB[3];
+        equalStatesAreStutter(subB[2],subB[3]);
+        assert StateNext(subB[2],subB[3]);
+        assert behaviorOutput(subB) == [Nil,Out(OperandContents(s,op1)),Out(OperandContents(s,op2)),Out(OperandContents(s,op2))];
+        assert sNext == evalInsRe(CALL(D(Void),stateOutputDump(op1,op2)),s);
+        assert sNext.ok;
+        var rest := evalBlockRE(stateOutputDump(op1,op2),s);
+        assert subB == [s] + rest;
+        assert behaviorOutput(rest) == [Out(OperandContents(s,op1)),Out(OperandContents(s,op2)),Out(OperandContents(s,op2))];
+        assert sNext.o == SubOut(behaviorOutput(rest));
+        return subB;
+    }
+
+
+
+    lemma equalStatesAreStutter(s:state,s':state)
+        requires s==s'
+        requires ValidState(s);
+        ensures ValidState(s');
+        ensures NextStep(s,s',Step.stutterStep());
+        ensures StateNext(s,s');
+    {
+         assert ValidState(s');
+         assert NextStep(s,s',Step.stutterStep());
+         assert StateNext(s,s');
+    }
+
+    lemma intsTypeMatch(x:Data,y:Data)
+        requires (isInt(x) && isInt(y))
+        requires x.itype.size == y.itype.size
+        requires x.itype.signed == y.itype.signed
+        ensures typesMatch(x,y);
+    {
+        assert typesMatch(x,y);
+    }
+
+    function validZero16bitInt(s:state) : (val:operand)
+        ensures val.D?;
+        ensures val.d.Int?;
+        ensures ValidData(s, val.d)
+        ensures !val.d.itype.signed
+        ensures val.d.itype.size == 4
+    {
+        var val := D(Int(0,IntType(4,false)));
+        assert  IntFits(val.d.val,val.d.itype);
+        val
+    }
+
+
+
+
+    predicate validPracticalBehavior(preB:behavior)
+    {
+        |preB| == 11
+
+        && ValidState(preB[0])
+        && ValidState(preB[1])
+        && ValidState(preB[2])
+        && ValidState(preB[3])
+        && ValidState(preB[4])
+        && ValidState(preB[5])
+        && ValidState(preB[6])
+        && ValidState(preB[7])
+        && ValidState(preB[8])
+        && ValidState(preB[9])
+        && ValidState(preB[10])
+        && StateNext(preB[0],preB[1])
+        && StateNext(preB[1],preB[2])
+        && StateNext(preB[0],preB[1])
+        && StateNext(preB[1],preB[2])
+        && StateNext(preB[2],preB[3])
+        && StateNext(preB[3],preB[4])
+        && StateNext(preB[4],preB[5])
+        && StateNext(preB[5],preB[6])
+        && StateNext(preB[6],preB[7])
+        && StateNext(preB[7],preB[8])
+        && StateNext(preB[8],preB[9])
+        && StateNext(preB[9],preB[10])
+    }
+
+    function validBehaviorsOuts():(validOut:seq<output>)
+    {
+        [Nil,
+        Nil,
+        Nil,
+        Nil,
+        Nil,
+        Nil,
+        Nil,
+        Nil,
+        Nil,
+        SubOut([Out((Int(16,IntType(4,false)))),Out(Int(4,IntType(1,false))),Out(Int(4,IntType(1,false)))]),
+        SubOut([Out((Int(16,IntType(4,false)))),Out(Int(4,IntType(1,false))),Out(Int(4,IntType(1,false)))])]
+    }
+
+    function validSideEffectBehaviorsOuts():(validOut:seq<output>)
+    {
+        [Nil,
+        Nil,
+        Nil,
+        Nil,
+        Nil,
+        Nil,
+        Nil,
+        Nil,
+        Nil,
+        SubOut([Out((Int(16,IntType(4,false)))),Out(Int(3,IntType(1,false))),Out(Int(3,IntType(1,false)))]),
+        SubOut([Out((Int(16,IntType(4,false)))),Out(Int(3,IntType(1,false))),Out(Int(3,IntType(1,false)))])]
+    }
+    
+
+}
