Dafny/examples/Challenge6/Challenge6PropertiesSideEffects.i.dfy
@@ -6,6 +6,7 @@ include "../../LLVM/behaviorLemmas.i.dfy"
 include "../../LLVM/llvmREFACTOR.i.dfy"
 include "../../LLVM/types.dfy"
 include "../../Libraries/Sets.i.dfy"
+include "Challenge6Common.i.dfy"
 
 module challenge6PropertiesSideEffects{
     import opened challenge6Code
@@ -16,6 +17,7 @@ module challenge6PropertiesSideEffects{
     import opened types
     import opened Collections__Sets_i
     import opened challenge6CodeLemmasPatchSideEffect
+    import opened challenge6common
 
         // benignPatch: "The patch does not add any NEW behaviors"
     predicate benignPatch(pre:set<behavior>,post:set<behavior>)
@@ -100,36 +102,6 @@ module challenge6PropertiesSideEffects{
         //     var b := unwrapPatchBehaviors(s,challenge_prob_6_code_write_encrypted_simple_patch_side_effect());
         //     assert behaviorOutput(postB) == validBehaviorsOuts();
         // }
-    }
-
-    function validBehaviorsOuts():(validOut:seq<output>)
-    {
-        [Nil,
-        Nil,
-        Nil,
-        Nil,
-        Nil,
-        Nil,
-        Nil,
-        Nil,
-        Nil,
-        SubOut([Out((Int(16,IntType(4,false)))),Out(Int(4,IntType(1,false))),Out(Int(4,IntType(1,false)))]),
-        SubOut([Out((Int(16,IntType(4,false)))),Out(Int(4,IntType(1,false))),Out(Int(4,IntType(1,false)))])]
-    }
-
-function validSideEffectBehaviorsOuts():(validOut:seq<output>)
-    {
-        [Nil,
-        Nil,
-        Nil,
-        Nil,
-        Nil,
-        Nil,
-        Nil,
-        Nil,
-        Nil,
-        SubOut([Out((Int(16,IntType(4,false)))),Out(Int(3,IntType(1,false))),Out(Int(3,IntType(1,false)))]),
-        SubOut([Out((Int(16,IntType(4,false)))),Out(Int(3,IntType(1,false))),Out(Int(3,IntType(1,false)))])]
     }
 
 
